experiment/Experiment.Steel.Notations.fst
@@ -2,25 +2,28 @@ module Experiment.Steel.Notations
 
 include Experiment.Steel.Interface
 
-module M  = Experiment.Steel.Repr.M
-module SE = Steel.Effect
+module M   = Experiment.Steel.Repr.M
+module SE  = Steel.Effect
+module SA  = Steel.Effect.Atomic
+module SH  = Experiment.Steel.SteelHack
+module Mem = Steel.Memory
 
 open FStar.Tactics
 open Experiment.Steel
 
 
 unfold
-let steel
-  : (a : Type) -> (pre : SE.pre_t) -> (post : SE.post_t a) ->
-    (req : SE.req_t pre) -> (ens : SE.ens_t pre a post) -> Type
-  = M.unit_steel
+let steel (a : Type) (pre : SE.pre_t) (post : SE.post_t a)
+          (req : SE.req_t pre) (ens : SE.ens_t pre a post)
+  : Type
+  = SH.unit_steel a pre post req ens
 
 unfold
 let to_steel
       (#a : Type) (#pre : SE.pre_t) (#post : SE.post_t a) (#req : SE.req_t pre) (#ens : SE.ens_t pre a post)
-      (t : M.repr a)
+      (t : M.repr SH.KSteel a)
       (g : __to_steel_goal a pre post req ens t)
-  : M.unit_steel a pre post req ens
+  : steel a pre post req ens
   = to_steel #a #pre #post #req #ens t g
 
 let mk_steel (fs : list flag) : Tac unit
@@ -29,33 +32,43 @@ let mk_steel (fs : list flag) : Tac unit
 
 unfold
 let return_hint (#a : Type) (x : a) (sl_hint : M.post_t a)
-  : M.repr a
+  : M.repr SH.KSteel a
   = M.return_hint #a x sl_hint
 
 unfold
 let return (#a : Type) (x : a)
-  : M.repr a
+  : M.repr SH.KSteel a
   = M.return #a x
 
+// TODO? generalize with typeclass
 unfold
-let bind (#a #b : Type) (f : M.repr a) (g : a -> M.repr b)
-  : M.repr b
+let bind (#a #b : Type) (f : M.repr SH.KSteel a) (g : a -> M.repr SH.KSteel b)
+  : M.repr SH.KSteel b
   = M.bind #a #b f g
 
 unfold
 let pure (#a : Type) (#wp : pure_wp a) ($f : unit -> PURE a wp)
-  : M.repr a
+  : M.repr SH.KSteel a
   = M.bindP wp f (fun x -> M.return x)
 
 unfold
-let ite (#a : Type) (guard : bool) (thn : M.repr a) (els : M.repr a)
-  : M.repr a
+let ite (#a : Type) (guard : bool) (thn : M.repr SH.KSteel a) (els : M.repr SH.KSteel a)
+  : M.repr SH.KSteel a
   = M.ite guard thn els
 
+/// Calling a Steel function from our representation
 unfold
 let call (#b : Type)
       (#a : b -> Type) (#pre : b -> SE.pre_t) (#post : (x : b) -> SE.post_t (a x))
       (#req : (x : b) -> SE.req_t (pre x)) (#ens : (x : b) -> SE.ens_t (pre x) (a x) (post x))
       ($f : (x : b) -> SE.Steel (a x) (pre x) (post x) (req x) (ens x)) (x : b)
-  : M.repr (a x)
+  : M.repr SH.KSteel (a x)
   = M.repr_of_steel (pre x) (post x) (req x) (ens x) (fun () -> f x)
+
+unfold
+let call_g (#b : Type)
+      (#a : b -> Type) (#opened : b -> Mem.inames) (#pre : b -> SE.pre_t) (#post : (x : b) -> SE.post_t (a x))
+      (#req : (x : b) -> SE.req_t (pre x)) (#ens : (x : b) -> SE.ens_t (pre x) (a x) (post x))
+      ($f : (x : b) -> SA.SteelGhost (a x) (opened x) (pre x) (post x) (req x) (ens x)) (x : b)
+  : M.repr (SH.KGhost (opened x)) (a x)
+  = M.repr_of_steel_ghost (pre x) (post x) (req x) (ens x) (fun () -> f x)
