experiment/Experiment.Steel.Test.Extract.fst
@@ -1,5 +1,6 @@
 module Experiment.Steel.Test.Extract
 
+module F    = Experiment.Steel.Notations
 module M    = Experiment.Steel.Repr.M
 module U32  = FStar.UInt32
 module Test = Experiment.Steel.Test
@@ -7,10 +8,14 @@ module Test = Experiment.Steel.Test
 open Steel.Effect
 open Steel.Reference
 
-
 let test3 (r0 r1 : ref U32.t)
   : Steel unit
-      (M.vprop_of_list' (Test.test3_mem r0 r1)) (fun _ -> M.vprop_of_list' (Test.test3_mem r0 r1))
+      (vptr r0 `star` vptr r1) (fun _ -> vptr r0 `star` vptr r1)
       (requires fun h0 -> U32.v (sel r0 h0) < 42)
       (ensures fun h0 () h1 -> U32.v (sel r1 h1) == U32.v (sel r0 h0) + 1)
   = Test.test3_steel' r0 r1 ()
+
+let test_ghost (r : ref U32.t)
+  : Steel U32.t (vptr r) (fun _ -> vptr r)
+      (requires fun _ -> True) (ensures fun h0 _ h1 -> frame_equalities (vptr r) h0 h1)
+  = Test.test_ghost r ()
